abstract_map.dfy
@@ -1,0 +1,97 @@
+module AppTypes {
+    datatype Datum = Datum(key:int, value:int)
+}
+
+module Log {
+import opened AppTypes
+
+datatype Constants = Constants()
+datatype Variables = Variables(ephemeral:imap<int, int>, persistent:imap<int, int>)
+
+predicate completeMap<K(!new),V>(a:imap<K,V>)
+{
+    forall k :: k in a
+}
+
+predicate WF(s:Variables)
+{
+    && completeMap(s.ephemeral)
+    && completeMap(s.persistent)
+}
+
+predicate InDomain(k:int)
+{
+    true
+}
+
+function ZeroMap() : (zmap : imap<int,int>)
+    ensures completeMap(zmap)
+{
+    imap k | InDomain(k) :: 0
+}
+
+predicate Init(k:Constants, s:Variables)
+    ensures Init(k, s) ==> WF(s);
+{
+    s == Variables(ZeroMap(), ZeroMap())
+}
+
+predicate Query(k:Constants, s:Variables, s':Variables, datum:Datum)
+    requires WF(s);
+{
+    && datum.value == s.ephemeral[datum.key]
+    && s' == s
+}
+
+predicate Write(k:Constants, s:Variables, s':Variables, datum:Datum)
+    requires WF(s);
+{
+    && s'.ephemeral == s.ephemeral[datum.key := datum.value]
+    && s'.persistent == s.persistent
+}
+
+// Report to the user that the disk is synchronized with the memory.
+predicate CompleteSync(k:Constants, s:Variables, s':Variables)
+    requires WF(s);
+{
+    && s.persistent == s.ephemeral
+    && s' == s
+}
+
+predicate SpontaneousUpdate(k:Constants, s:Variables, s':Variables, key:int)
+    requires WF(s);
+{
+    && s'.ephemeral == s.ephemeral
+    && s'.persistent == s.persistent[key := s.ephemeral[key]]
+}
+
+// Forget all non-persisted data.
+predicate SpontaneousCrash(k:Constants, s:Variables, s':Variables)
+    requires WF(s);
+{
+    && s'.ephemeral == s.persistent
+    && s'.persistent == s.persistent
+}
+
+datatype Step = Query(datum:Datum) | Write(datum:Datum) | CompleteSync | SpontaneousUpdate(key:int) | SpontaneousCrash
+
+predicate NextStep(k:Constants, s:Variables, s':Variables, step:Step)
+    requires WF(s);
+{
+    match step {
+        case Query(datum) => Query(k, s, s', datum)
+        case Write(datum) => Write(k, s, s', datum)
+        case CompleteSync() => CompleteSync(k, s, s')
+        case SpontaneousUpdate(key) => SpontaneousUpdate(k, s, s', key)
+        case SpontaneousCrash() => SpontaneousCrash(k, s, s')
+    }
+}
+
+predicate Next(k:Constants, s:Variables, s':Variables)
+    requires WF(s);
+    ensures Next(k, s, s') ==> WF(s');
+{
+    exists step :: NextStep(k, s, s', step)
+}
+
+}
